Main.lean
@@ -5,13 +5,15 @@ import LeanUpdate.CreateIssue
 import LeanUpdate.FindDep
 import LeanUpdate.UpdateDependencies
 import LeanUpdate.UpdateLeanToolchain
+import LeanUpdate.PostUpdateValidation
 
 public def main (args : List String) : IO Unit := do
   match args with
   | ["checkChanges"] => runCheckChanges
-  | ["createIssue", "success"] => runCreateIssue .success
-  | ["createIssue", "failure"] => runCreateIssue .failure
+  | ["createIssue"] => runCreateIssue
   | ["findDependencies"] => runFindDependencies
   | ["updateDependencies"] => runUpdateDependencies
   | ["updateLeanToolchain"] => runUpdateLeanToolchain
+  | ["validateUpdate"] =>
+    let _ ← runPostUpdateValidation
   | _ => throw <| IO.userError "invalid arguments of leanUpdate"
